theories/SimplyTypedLambdaCalculus/StrongNormalisation.v
@@ -1,20 +1,28 @@
 From FormArith.SimplyTypedLambdaCalculus Require Import Definitions.
 
+Require Import Relations.Relations.
+
 
 Inductive SN: term -> Prop :=
   | Strong (t: term) :
       (forall (t': term), t ~> t' -> SN t') -> SN t.
+
+Locate "~>*".
 
 Fixpoint reducible (A: type) (t: term): Prop :=
   match A with
   | Base => SN t
   | Arr A B => forall (u: term), reducible A u -> reducible B (App t u)
   | Prod A B => reducible A (Pr1 t) /\ reducible B (Pr2 t)
+  | Sum A B =>
+      SN t /\
+      (forall u, t ~>* In1 u -> reducible A u) /\
+      (forall v, t ~>* In2 v -> reducible B v)
   end.
 
 Definition neutral (t: term): Prop :=
   match t with
-  | Lam _ | Pair _ _ => False
+  | Lam _ | Pair _ _ | In1 _ | In2 _ => False
   | _ => True
   end.
 
@@ -25,8 +33,12 @@ Inductive sub_term: term -> term -> Prop :=
   | Sub_pair1 (t1 t2: term): sub_term t1 (Pair t1 t2)
   | Sub_pair2 (t1 t2: term): sub_term t2 (Pair t1 t2)
   | Sub_pr1 (t: term): sub_term t (Pr1 t)
-  | Sub_pr2 (t: term): sub_term t (Pr2 t).
-
+  | Sub_pr2 (t: term): sub_term t (Pr2 t)
+  | Sub_pat1 (t1 t2 t3: term): sub_term t1 (Pat t1 t2 t3)
+  | Sub_pat2 (t1 t2 t3: term): sub_term t2 (Pat t1 t2 t3)
+  | Sub_pat3 (t1 t2 t3: term): sub_term t3 (Pat t1 t2 t3)
+  | Sub_in1 (t: term): sub_term t (In1 t)
+  | Sub_in2 (t: term): sub_term t (In2 t).
 
 Lemma SN_lam (t: term):
   SN t -> SN (Lam t).
@@ -51,6 +63,7 @@ Proof.
        | H: _ |- _ => idtac
        end.
 
+  (** Classical Lambda calculus *)
   - apply IH with (App u t2).
     + now apply Beta_AppL.
     + apply Sub_app1.
@@ -63,6 +76,7 @@ Proof.
     + now apply Beta_Lam.
     + apply Sub_lam.
 
+  (** Pairs and projections *)
   - apply IH with (Pair u t2).
     + now apply Beta_Pair1.
     + apply Sub_pair1.
@@ -78,6 +92,27 @@ Proof.
   - apply IH with (Pr2 u).
     + now apply Beta_Pr2.
     + apply Sub_pr2.
+
+  (** Sum types *)
+  - apply IH with (Pat u t2 t3).
+    + now apply Beta_Pat1.
+    + apply Sub_pat1.
+
+  - apply IH with (Pat t1 u t3).
+    + now apply Beta_Pat2.
+    + apply Sub_pat2.
+
+  - apply IH with (Pat t1 t2 u).
+    + now apply Beta_Pat3.
+    + apply Sub_pat3.
+
+  - apply IH with (In1 u).
+    + now apply Beta_In1.
+    + apply Sub_in1.
+
+  - apply IH with (In2 u).
+    + now apply Beta_In2.
+    + apply Sub_in2.
 Qed.
 
 Lemma SN_var_app (t: term) (n: var):
@@ -101,7 +136,8 @@ Lemma reducible_is_SN (A : type):
 Proof.
   induction A as [
     | A [IHA1 [IHA2 IHA3]] B [IHB1 [IHB2 IHB3]]
-    | A [IHA1 [IHA2 IHA3]] B [IHB1 [IHB2 IHB3]] ].
+    | A [IHA1 [IHA2 IHA3]] B [IHB1 [IHB2 IHB3]]
+    | A [IHA1 [IHA2 IHA3]] B [IHB1 [IHB2 IHB3]]].
   - do 3 split.
     + intros.
       apply SN_inverted with t'; [| assumption ].
@@ -157,6 +193,27 @@ Proof.
         apply (H s' H1).
       * apply IHB3; [ exact I | ]. intros t' Hstep. inv Hstep; [| destruct Hneu ].
         apply (H s' H1).
+
+  - split; [| split]; simpl.
+    + intros t [HSN _]. apply HSN.
+
+    + intros t u [Hredt1 [Hredt2 Hredt3]] Hbeta. split; [| split].
+      * apply (SN_inverted t Hredt1). assumption.
+      * intros. apply Hredt2.
+        apply rt_trans with u; [| assumption ].
+        now apply rt_step.
+      * intros. apply Hredt3.
+        apply rt_trans with u; [| assumption ].
+        now apply rt_step.
+
+    + intros t Hneu H. split; [| split ].
+      * apply Strong. intros t' ?. apply H. assumption.
+      * intros u Hbeta. rewrite clos_rt_rt1n_iff in Hbeta.
+        inv Hbeta; [ destruct Hneu |].
+        apply H with y; [ assumption |]. apply clos_rt_rt1n_iff. assumption.
+      * intros u Hbeta. rewrite clos_rt_rt1n_iff in Hbeta.
+        inv Hbeta; [ destruct Hneu |].
+        apply H with y; [ assumption |]. apply clos_rt_rt1n_iff. assumption.
 Qed.
 
 Lemma SN_subst (t: term) (σ: var -> term):
@@ -189,6 +246,35 @@ Proof.
   - now apply IHv.
   - apply IHt; [ assumption |].
     now apply Strong.
+Qed.
+
+Lemma SN_triple_ind (P : term -> term -> term -> Prop):
+  (forall t u v, (forall t' u' v',
+                ((t = t' /\ u = u' /\ v ~> v') \/
+                   (t = t' /\ u ~> u' /\ v = v') \/
+                   (t ~> t' /\ u = u' /\ v = v'))
+                -> P t' u' v') -> P t u v)
+    -> forall t u v, SN t -> SN u -> SN v -> P t u v.
+Proof.
+  intros IH t u v Hsnt.
+  revert u v.
+
+  induction Hsnt as [? _ IHt].
+  intros u v Hsnu. revert v.
+  induction Hsnu as [? HSNu IHu].
+  intros v Hsnv.
+  induction Hsnv as [? HSNv IHv].
+  apply IH.
+
+  intros ? ? ? [[? [? ?]] | [[? [? ?]] | [? [? ?]]]]; subst.
+  - now apply IHv.
+  - apply IHu.
+    + assumption.
+    + apply Strong. intros. now apply HSNv.
+  - apply IHt.
+    + assumption.
+    + apply Strong. intros. now apply HSNu.
+    + apply Strong. intros. now apply HSNv.
 Qed.
 
 Lemma reducible_abs (v: term) (A B: type):
@@ -281,6 +367,108 @@ Proof.
     + assumption.
 Qed.
 
+Lemma reducible_sum1 (A B: type) (s: term):
+  reducible A s ->
+  reducible (Sum A B) (In1 s).
+Proof.
+  intros Hreds. simpl.
+  specialize (reducible_is_SN A) as (HA1 & HA2 & HA3).
+  assert (HSN: SN s) by now apply HA1.
+  induction HSN as [s _ IH]. split.
+  - apply Strong. intros t' Hstep. inv Hstep. apply IH.
+    + assumption.
+    + now apply HA2 with s.
+  - split.
+    + intros u Hbeta; rewrite clos_rt_rt1n_iff in Hbeta;
+      inv Hbeta; [ assumption |]. inv H.
+      apply (IH s').
+      * assumption.
+      * now apply (HA2 s).
+      * now apply clos_rt_rt1n_iff.
+    + intros v Hbeta. rewrite clos_rt_rt1n_iff in Hbeta;
+        inv Hbeta. inv H.
+      apply (IH s').
+      * assumption.
+      * now apply (HA2 s).
+      * now apply clos_rt_rt1n_iff.
+Qed.
+
+Lemma reducible_sum2 (A B: type) (s: term):
+  reducible B s ->
+  reducible (Sum A B) (In2 s).
+Proof.
+  intros Hreds. simpl.
+  specialize (reducible_is_SN B) as (HB1 & HB2 & HB3).
+  assert (HSN: SN s) by now apply HB1.
+  induction HSN as [s _ IH]. split.
+  - apply Strong. intros t' Hstep. inv Hstep. apply IH.
+    + assumption.
+    + now apply HB2 with s.
+  - split.
+    + intros u Hbeta; rewrite clos_rt_rt1n_iff in Hbeta;
+      inv Hbeta. inv H.
+      apply (IH s').
+      * assumption.
+      * now apply (HB2 s).
+      * now apply clos_rt_rt1n_iff.
+    + intros v Hbeta. rewrite clos_rt_rt1n_iff in Hbeta;
+        inv Hbeta; [ assumption |]. inv H.
+      apply (IH s').
+      * assumption.
+      * now apply (HB2 s).
+      * now apply clos_rt_rt1n_iff.
+Qed.
+
+Lemma reducible_pat (A B C: type) (t u v: term):
+  reducible (Sum A B) t ->
+  reducible (Arr A C) (Lam u) ->
+  reducible (Arr B C) (Lam v) ->
+  reducible C (Pat t u v).
+Proof.
+  intros Hredt Hredu Hredv.
+  specialize (reducible_is_SN (Arr A C)) as (HAC1 & HAC2 & HAC3).
+  specialize (reducible_is_SN (Arr B C)) as (HBC1 & HBC2 & HBC3).
+  specialize (reducible_is_SN (Sum A B)) as (H1 & H2 & H3).
+  specialize (reducible_is_SN C) as (HC1 & HC2 & HC3).
+
+  assert (HSNt: SN t) by now apply H1.
+  assert (HSNu: SN u). {
+    apply SN_sub_term with (Lam u).
+    - apply HAC1. assumption.
+    - apply Sub_lam.
+  }
+
+  assert (HSNv: SN v). {
+    apply SN_sub_term with (Lam v).
+    - apply HBC1. assumption.
+    - apply Sub_lam.
+  }
+
+  revert Hredt Hredu Hredv. apply SN_triple_ind with (t := t) (u := u) (v := v).
+  2, 3, 4: assumption.
+  intros t0 u0 v0 IH Hredt0 Hredu0 Hredv0. apply HC3; [ exact I |].
+  intros t' Hstep. inv Hstep.
+  - apply IH; try assumption.
+    + right. now right.
+    + apply H2 with t0; assumption.
+  - apply IH; try assumption.
+    + right. now left.
+    + apply HAC2 with (Lam u0); [ assumption | now apply Beta_Lam ].
+  - apply IH; try assumption.
+    + now left.
+    + apply HBC2 with (Lam v0); [ assumption | now apply Beta_Lam ].
+  - enough (reducible C (App (Lam u0) t1)).
+    + apply HC2 with (App (Lam u0) t1).
+      * assumption.
+      * now apply Beta_Subst.
+    + simpl in Hredu0. apply Hredu0. apply Hredt0. apply rt_refl.
+  - enough (reducible C (App (Lam v0) t1)).
+    + apply HC2 with (App (Lam v0) t1).
+      * assumption.
+      * now apply Beta_Subst.
+    + simpl in Hredv0. apply Hredv0. apply Hredt0. apply rt_refl.
+Qed.
+
 Lemma typing_is_reducible (Γ: var -> type) (σ: var -> term):
   (forall (x: var), reducible (Γ x) (σ x)) ->
     forall (A: type) (t: term), Γ ⊢ t : A -> reducible A t.[σ].
@@ -290,7 +478,7 @@ Proof.
   revert σ A Γ.
 
   induction t; intros σ A Γ Hred.
-  all: inversion 1; subst; simpl.
+  all: inversion 1; subst.
 
   - apply Hred.
   - apply IHt1 with (σ := σ) in H2; [| assumption ].
@@ -308,6 +496,18 @@ Proof.
 
   - apply (IHt σ (Prod A B) Γ Hred H1).
   - apply (IHt σ (Prod A0 A) Γ Hred H1).
+
+  - simpl. apply reducible_pat with A0 B.
+    + now apply IHt with Γ.
+    + apply reducible_abs. intros u0 Hredu0.
+      asimpl. apply IHt0 with (A0 .: Γ); [| assumption ].
+      intros [| x ]; simpl; [ assumption | apply Hred ].
+    + apply reducible_abs. intros. asimpl. apply IHt1 with (B .: Γ); [| assumption ].
+      intros [| x ]; simpl; [ assumption | apply Hred ].
+  - change (reducible (Sum A0 B) (In1 t.[σ])).
+    apply reducible_sum1. now apply IHt with Γ.
+  - change (reducible (Sum A0 B) (In2 t.[σ])).
+    apply reducible_sum2. now apply IHt with Γ.
 Qed.
 
 Corollary STLC_is_SN (A: type) (Γ: var -> type) (t: term):
